src/guarding/tactics.v
@@ -1,0 +1,213 @@
+Require Import guarding.guard.
+From iris.prelude Require Import options.
+
+Section TacticsHelpers.
+
+Context {Σ: gFunctors}.
+Context `{!invGS Σ}. 
+ 
+Local Lemma guard_weaken_helper_right (A B C : iProp Σ) (E: coPset) (n: nat)
+    : (A &&{E; n}&&> B) -∗ (B &&{E}&&> C) -∗ (A &&{E; n}&&> C).
+Proof.
+  iIntros "x y". iDestruct (lguards_transitive _ A B C with "[x y]") as "z".
+  - iFrame "x". iFrame "y". - replace (n + 0) with n by trivial. iFrame "z".
+Qed.
+
+Local Lemma guard_weaken_helper_right_laters_plus (A B C : iProp Σ) (E: coPset) (n m: nat)
+    : (A &&{E; n}&&> B) -∗ (B &&{E; m}&&> C) -∗ (A &&{E; n + m}&&> C).
+Proof.
+  iIntros "x y". iDestruct (lguards_transitive _ A B C with "[x y]") as "z".
+  - iFrame "x". iFrame "y". - replace (n + 0) with n by trivial. iFrame "z".
+Qed.
+
+Local Lemma guard_weaken_helper_left (A B C : iProp Σ) (E: coPset) (n: nat)
+    : (B &&{E; n}&&> C) -∗ (A &&{E}&&> B) -∗ (A &&{E; n}&&> C).
+Proof.
+  iIntros "x y". iDestruct (lguards_transitive _ A B C with "[x y]") as "z".
+  - iFrame "x". iFrame "y". - replace (0 + n) with n by trivial. iFrame "z".
+Qed.
+
+Local Lemma guard_weaken_helper_left_laters_plus (A B C : iProp Σ) (E: coPset) (n m: nat)
+    : (B &&{E; n}&&> C) -∗ (A &&{E; m}&&> B) -∗ (A &&{E; n + m}&&> C).
+Proof.
+  iIntros "x y". iDestruct (lguards_transitive _ A B C with "[x y]") as "z".
+  - iFrame "x". iFrame "y". - replace (n + m) with (m + n) by lia. iFrame "z".
+Qed.
+ 
+Local Lemma guard_goal_helper_right (A B C : iProp Σ) (E: coPset) (n: nat)
+    : (A &&{E}&&> B) -∗ (B &&{E; n}&&> C) -∗ (A &&{E; n}&&> C).
+Proof.
+  iIntros "x y". iDestruct (lguards_transitive _ A B C with "[x y]") as "z".
+  - iFrame "x". iFrame "y". - replace (0 + n) with (n) by lia. iFrame "z".
+Qed.
+
+Local Lemma guard_goal_helper_left (A B C : iProp Σ) (E: coPset) (n: nat)
+    : (B &&{E}&&> C) -∗ (A &&{E; n}&&> B) -∗ (A &&{E; n}&&> C).
+Proof.
+  iIntros "x y". iDestruct (lguards_transitive _ A B C with "[x y]") as "z".
+  - iFrame "x". iFrame "y". - replace (n + 0) with (n) by trivial. iFrame "z".
+Qed.
+
+Local Lemma guard_goal_helper_right_laters_minus (A B C : iProp Σ) (E: coPset) (n m: nat)
+  (le: m ≤ n)
+    : (A &&{E; m}&&> B) -∗ (B &&{E; n-m}&&> C) -∗ (A &&{E; n}&&> C).
+Proof.
+  iIntros "x y". iDestruct (lguards_transitive _ A B C with "[x y]") as "z".
+  - iFrame "x". iFrame "y". - replace (m + (n-m)) with (n) by lia. iFrame "z".
+Qed.
+
+Local Lemma guard_goal_helper_left_laters_minus (A B C : iProp Σ) (E: coPset) (n m: nat)
+  (le: m ≤ n)
+    : (B &&{E; m}&&> C) -∗ (A &&{E; n-m}&&> B) -∗ (A &&{E; n}&&> C).
+Proof.
+  iIntros "x y". iDestruct (lguards_transitive _ A B C with "[x y]") as "z".
+  - iFrame "x". iFrame "y". - replace (n - m + m) with (n) by lia. iFrame "z".
+Qed.
+
+Local Lemma lguards_open_helper (P Q : iProp Σ) (E F : coPset) n
+    (su: F ⊆ E)
+    : (P &&{F; n}&&> Q) -∗ P ={E, E ∖ F}=∗
+      ▷^n |={E ∖ F}=> (Q ∗ (Q ={E ∖ F, E}=∗ P)).
+Proof.
+  iIntros "x y". iApply lguards_open; trivial. iFrame.
+Qed.
+
+Local Lemma guards_open_helper (P Q : iProp Σ) (E F : coPset)
+    (su: F ⊆ E)
+    : (P &&{F}&&> Q) -∗ P ={E, E ∖ F}=∗
+      (Q ∗ (Q ={E ∖ F, E}=∗ P)).
+Proof.
+  iIntros "x y". iApply guards_open; trivial. iFrame.
+Qed.
+
+
+End TacticsHelpers.
+
+Tactic Notation "leaf_hyp" constr(g1) "rhs" "to" open_constr(Q) "as" constr(g2) :=
+  iPoseProof (guard_weaken_helper_right _ _ Q with (append g1 " []")) as g2.
+  
+Tactic Notation "leaf_hyp" constr(g1) "rhs" "to" open_constr(Q) "laters" "plus" open_constr(n) "as" constr(g2) :=
+  iPoseProof (guard_weaken_helper_right_laters_plus _ _ Q _ _ n with (append g1 " []")) as g2.
+  
+Tactic Notation "leaf_hyp" constr(g1) "lhs" "to" open_constr(Q) "as" constr(g2) :=
+  iPoseProof (guard_weaken_helper_left Q with (append g1 " []")) as g2.
+  
+Tactic Notation "leaf_hyp" constr(g1) "lhs" "to" open_constr(Q) "laters" "plus" open_constr(n) "as" constr(g2) :=
+  iPoseProof (guard_weaken_helper_left_laters_plus Q _ _ _ _ n with (append g1 " []")) as g2.
+  
+Tactic Notation "leaf_hyp" constr(g1) "mask" "to" open_constr(E) "as" constr(g2) :=
+  iPoseProof (lguards_mask_weaken _ _ _ E with g1) as g2.
+  
+Tactic Notation "leaf_hyp" constr(g1) "laters" "to" open_constr(n) "as" constr(g2) :=
+  iPoseProof (lguards_weaken_later _ _ _ _ n with g1) as g2.
+  
+Tactic Notation "leaf_goal" "rhs" "to" open_constr(Q) :=
+  iApply (guard_goal_helper_left _ Q).
+  
+Tactic Notation "leaf_goal" "lhs" "to" open_constr(Q) "laters" "minus" open_constr(n) :=
+  iApply (guard_goal_helper_right_laters_minus _ Q _ _ _ n).
+  
+Tactic Notation "leaf_goal" "rhs" "to" open_constr(Q) "laters" "minus" open_constr(n) :=
+  iApply (guard_goal_helper_left_laters_minus _ Q _ _ _ n).
+  
+Tactic Notation "leaf_goal" "lhs" "to" open_constr(Q) :=
+  iApply (guard_goal_helper_right _ Q).
+  
+Tactic Notation "leaf_goal" "mask" "to" open_constr(E) :=
+  iApply (lguards_mask_weaken _ _ E).
+  
+Tactic Notation "leaf_goal" "laters" "to" open_constr(n) :=
+  iApply (lguards_weaken_later _ _ _ n).
+  
+Tactic Notation "leaf_by_sep" :=
+  iApply lguards_weaken; iModIntro.
+  
+Tactic Notation "leaf_by_sep_except0" :=
+  iApply lguards_weaken_except0; iModIntro.
+  
+Tactic Notation "leaf_open" constr(g) "with" constr(sel) "as" constr(pat) :=
+  iMod (guards_open_helper with (append g (append " " sel))) as pat.
+   
+Tactic Notation "leaf_open_laters" constr(g) "with" constr(sel) "as" constr(pat) :=
+  iMod (lguards_open_helper with (append g (append " " sel))) as pat.
+
+  
+Context {Σ: gFunctors}.
+Context `{!invGS Σ}. 
+ 
+Section TacticsTests.
+  
+Local Lemma test_leaf_hyp (A B C D : iProp Σ) E
+    : (A &&{∅ ; 3}&&> B ∗ C) ⊢ (A ∗ D &&{E ; 20}&&> B).
+Proof.
+  iIntros "g".
+  leaf_hyp "g" rhs to (B) as "g1".
+    { leaf_by_sep. iIntros "[b c]". iFrame. iIntros. done. }
+  leaf_hyp "g1" lhs to (A ∗ D)%I as "g2".
+    { leaf_by_sep. iIntros "[a d]". iFrame. iIntros. done. }
+  leaf_hyp "g2" mask to E as "g3". { set_solver. }
+  leaf_hyp "g3" laters to 20 as "g4". { lia. }
+  iFrame.
+Qed.
+
+Local Lemma test_leaf_hyp2 (A B C D : iProp Σ)
+    : (A &&{∅ ; 3}&&> B ∗ C) ⊢ (A ∗ D &&{∅ ; 20}&&> B).
+Proof.
+  iIntros "g".
+  leaf_hyp "g" rhs to (B) laters plus 2 as "g1".
+    { leaf_by_sep. iIntros "[b c]". iModIntro. iModIntro. iFrame. iIntros. done. }
+  leaf_hyp "g1" lhs to (A ∗ D)%I laters plus 4 as "g2".
+    { leaf_by_sep. iIntros "[a d]". iFrame. iModIntro. iModIntro. iModIntro. iModIntro. iIntros. done. }
+  leaf_hyp "g2" laters to 20 as "g4". { lia. }
+  iFrame.
+Qed.
+
+Local Lemma test_leaf_goal (A B C D : iProp Σ) E
+    : (A &&{∅ ; 3}&&> B ∗ C) ⊢ (A ∗ D &&{E ; 20}&&> B).
+Proof.
+  iIntros.
+  leaf_goal rhs to (B ∗ C)%I.
+    { leaf_by_sep. iIntros "[b c]". iFrame. iIntros. done. }
+  leaf_goal lhs to (A)%I.
+    { leaf_by_sep_except0. iIntros "[a d]". iModIntro. iFrame. iIntros. done. }
+  leaf_goal mask to ∅. { set_solver. }
+  leaf_goal laters to 3. { lia. }
+  iFrame "#".
+Qed.
+
+Local Lemma test_leaf_goal2 (A B C D : iProp Σ) E
+    : (A &&{∅ ; 3}&&> B ∗ C) ⊢ (A ∗ D &&{E ; 20}&&> B).
+Proof.
+  iIntros "#g".
+  leaf_goal lhs to (A)%I laters minus 1. { lia. }
+    { leaf_by_sep. iIntros "[b c]". iModIntro. iFrame. iIntros. done. }
+  leaf_goal rhs to (B ∗ C)%I laters minus 3. { lia. }
+    { leaf_by_sep. iIntros "[b c]". iModIntro. iModIntro. iModIntro. iFrame. iIntros. done. }
+  leaf_goal mask to ∅. { set_solver. }
+  leaf_goal laters to 3. { lia. }
+  iFrame "#".
+Qed.
+
+Local Lemma test_leaf_open (A B C D : iProp Σ) E
+    : (A &&{E}&&> □(B → C)) ∗ A ∗ B ={E}=∗ C.
+Proof.
+  iIntros "[#g [a b]]".
+  leaf_open "g" with "a" as "[#bc back]". { set_solver. }
+  iDestruct ("bc" with "b") as "c".
+  iMod ("back" with "[bc]") as "j". { iModIntro. iFrame "#". }
+  iModIntro. iFrame.
+Qed.
+  
+Local Lemma test_leaf_open2 (A B C D : iProp Σ) E n
+    : (A &&{E; n}&&> □(B → C)) ∗ A ∗ B ⊢ |={E,∅}=> ▷^n |={∅,E}=> C.
+Proof.
+  iIntros "[#g [a b]]".
+  leaf_open_laters "g" with "a" as "lats". { set_solver. }
+  replace (E ∖ E) with (∅ : coPset) by set_solver.
+  iModIntro. iNext. iMod "lats" as "[#bc back]".
+  iDestruct ("bc" with "b") as "c".
+  iMod ("back" with "[bc]") as "j". { iModIntro. iFrame "#". }
+  iModIntro. iFrame.
+Qed.
+
+End TacticsTests.
