tactics.md
@@ -1,0 +1,115 @@
+# Tactics
+
+Leaf supplies various tactics for use in Iris Proof Mode.
+
+`src/guarding/tactics.v` provides example uses of these tactics.
+
+### `leaf_hyp`
+
+`leaf_hyp` makes it easy to use a guard proposition from the context
+to produce a related guard proposition.
+It takes one of the following forms:
+
+```
+leaf_hyp "H" lhs to P' as "G".
+leaf_hyp "H" rhs to Q' as "G".
+leaf_hyp "H" mask to E' as "G".
+leaf_hyp "H" laters to n' as "G".
+```
+
+Assuming that `"H"` is a proposition in the persistent context
+of the form `P &&{ E; n }&&> Q` or `P &&{ E }&&> Q`.
+The idea is that you specify a guard proposition and which element you
+want to modify, either:
+
+ * The lhs, weakening it to `P'`. This creates a subgoal `P' &&{E}&&> P`.
+ * The rhs, weakening it to `Q'`. This creates a subgoal `Q &&{E}&&> Q'`.
+ * The mask, weakening it to `E'`. This creates a subgoal `E ⊆ E'`
+ * The later-count, weakening it to `n'`. This creates a subgoal `n ≤ n'`
+
+It places the resulting weakened guard proposition in the persistent context
+with the specified name (here `"G'`).
+
+When operating on the lhs or rhs, you can also weaken the later count at the same time.
+
+```
+leaf_hyp "H" lhs to P' laters plus m as "G".
+leaf_hyp "H" rhs to Q' laters plus m as "G".
+```
+
+The first creates a subgoal `P' &&{ E; m }&&> P`,
+and produces `P' &&{ e; n + m }&&> Q`.
+
+Likewise for the rhs, it creates a subgoal `Q &&{ E; m }&&> Q'`
+and produces `P &&{ e; n + m }&&> Q'`.
+
+### `leaf_goal`
+
+Similar to the above, except it strengthens the goal rather than weakens a hypothesis.
+
+```
+leaf_goal lhs to P'.
+leaf_goal rhs to Q'.
+leaf_goal mask to E'.
+leaf_goal laters to n'.
+```
+
+Again, you specify a particular element of the proposition and specify what you want
+to change that element to:
+
+ * The lhs, strengthening it to `P'`. This creates a subgoal `P &&{E}&&> P'`.
+ * The rhs, strengthening it to `Q'`. This creates a subgoal `Q' &&{E}&&> Q`.
+ * The mask, strengthening it to `E'`. This creates a subgoal `E' ⊆ E`
+ * The later-count, strengthening it to `n'`. This creates a subgoal `n' ≤ n`
+
+Again, you can modify the later count while operating on the lhs and rhs.
+This time, the later-count decreases:
+
+```
+leaf_hyp "H" lhs to P' laters minus m as "G".
+leaf_hyp "H" rhs to Q' laters minus m as "G".
+```
+
+### `leaf_by_sep`
+
+```
+leaf_by_sep.
+```
+
+When the goal is `P &&{E}&&> Q`,
+the `leaf_by_sep` tactic reduces it to a goal `□ (P -∗ (Q ∗ (Q -∗ P)))`.
+
+This is useful when:
+
+ * Your goal is `P &&{E}&&> Q`, where `P ⊣⊢ Q`
+ * Your goal is `(A ∗ B) &&{E}&&> A` 
+ * Your goal is `P &&{E}&&> Q`, where `P` and `Q` are equivalent under assumptions
+    in the persistent context.
+
+When the goal is `P &&{ E ; n }&&> Q`, the goal becomes
+`P -∗ ▷^n (Q ∗ (Q -∗ P))`.
+
+### `leaf_by_sep_except0`
+
+```
+leaf_by_sep_except0.
+```
+
+This is like `leaf_by_sep` except it produces the goal with an extra except-0 modality:
+`P -∗ ▷^n ◇ (Q ∗ (Q -∗ P))`.
+
+This is useful if you want to remove laters from timeless propositions. E.g., you can show
+`P &&{E}&&> ▷ P` for timeless `P` this way.
+
+### `leaf_open` and `leaf_open_laters`
+
+Wrapper around `guards_open` and `lguards_open`.
+
+```
+leaf_open "G" with "A" as "X"
+leaf_open_laters "G" with "A" as "X"
+```
+
+ * `"G"` is the name of guards proposition, say `"G": P &&{E}&&> Q`. 
+ * `"A"` is a specialization pattern used to fulfill the `P` obligation.
+ * `"X"` is an introduction pattern where the resulting `Q` goes.
